coq/CoqOfSolidity/contracts/erc20/erc20_shallow.v
@@ -10,7 +10,7 @@ Module Erc20_403.
       let_state~ 'tt := [[
         Shallow.if_ (|
           gt ~(| x, sum |),
-          do~ [[ mstore ~(| 0, (shl ~(| 224, 0x4e487b71 |)) |) ]] in
+          do~ [[ mstore ~(| 0, shl ~(| 224, 0x4e487b71 |) |) ]] in
           do~ [[ mstore ~(| 4, 0x11 |) ]] in
           do~ [[ revert ~(| 0, 0x24 |) ]] in
           M.pure (BlockUnit.Tt, tt),
@@ -35,29 +35,29 @@ Module Erc20_403.
       ]] default~ tt in
       let_state~ 'tt := [[
         Shallow.if_ (|
-          iszero ~(| (caller ~(||)) |),
-          do~ [[ mstore ~(| _1, (shl ~(| 229, 4594637 |)) |) ]] in
-          do~ [[ mstore ~(| (add ~(| _1, 4 |)), 32 |) ]] in
-          do~ [[ mstore ~(| (add ~(| _1, 36 |)), 31 |) ]] in
-          do~ [[ mstore ~(| (add ~(| _1, 68 |)), 0x45726332303a206d696e7420746f20746865207a65726f206164647265737300 (* Erc20: mint to the zero address *) |) ]] in
+          iszero ~(| caller ~(||) |),
+          do~ [[ mstore ~(| _1, shl ~(| 229, 4594637 |) |) ]] in
+          do~ [[ mstore ~(| add ~(| _1, 4 |), 32 |) ]] in
+          do~ [[ mstore ~(| add ~(| _1, 36 |), 31 |) ]] in
+          do~ [[ mstore ~(| add ~(| _1, 68 |), 0x45726332303a206d696e7420746f20746865207a65726f206164647265737300 (* Erc20: mint to the zero address *) |) ]] in
           do~ [[ revert ~(| _1, 100 |) ]] in
           M.pure (BlockUnit.Tt, tt),
           tt
         |)
       ]] default~ tt in
-      do~ [[ sstore ~(| 0x02, (checked_add_uint256 ~(| (sload ~(| 0x02 |)) |)) |) ]] in
-      do~ [[ mstore ~(| 0x00, (caller ~(||)) |) ]] in
+      do~ [[ sstore ~(| 0x02, checked_add_uint256 ~(| sload ~(| 0x02 |) |) |) ]] in
+      do~ [[ mstore ~(| 0x00, caller ~(||) |) ]] in
       do~ [[ mstore ~(| 0x20, 0x00 |) ]] in
-      let~ _2 := [[ checked_add_uint256 ~(| (sload ~(| (keccak256 ~(| 0x00, 64 |)) |)) |) ]] in
-      do~ [[ mstore ~(| 0x00, (caller ~(||)) |) ]] in
+      let~ _2 := [[ checked_add_uint256 ~(| sload ~(| keccak256 ~(| 0x00, 64 |) |) |) ]] in
+      do~ [[ mstore ~(| 0x00, caller ~(||) |) ]] in
       do~ [[ mstore ~(| 0x20, 0x00 |) ]] in
-      do~ [[ sstore ~(| (keccak256 ~(| 0x00, 64 |)), _2 |) ]] in
+      do~ [[ sstore ~(| keccak256 ~(| 0x00, 64 |), _2 |) ]] in
       let~ _3 := [[ mload ~(| 64 |) ]] in
       do~ [[ mstore ~(| _3, 0x14 |) ]] in
-      do~ [[ log3 ~(| _3, 0x20, 0xddf252ad1be2c89b69c2b068fc378daa952ba7f163c4a11628f55a4df523b3ef, 0x00, (caller ~(||)) |) ]] in
+      do~ [[ log3 ~(| _3, 0x20, 0xddf252ad1be2c89b69c2b068fc378daa952ba7f163c4a11628f55a4df523b3ef, 0x00, caller ~(||) |) ]] in
       let~ _4 := [[ mload ~(| 64 |) ]] in
       let~ _5 := [[ datasize ~(| 0x45726332305f3430335f6465706c6f7965640000000000000000000000000000 (* Erc20_403_deployed *) |) ]] in
-      do~ [[ codecopy ~(| _4, (dataoffset ~(| 0x45726332305f3430335f6465706c6f7965640000000000000000000000000000 (* Erc20_403_deployed *) |)), _5 |) ]] in
+      do~ [[ codecopy ~(| _4, dataoffset ~(| 0x45726332305f3430335f6465706c6f7965640000000000000000000000000000 (* Erc20_403_deployed *) |), _5 |) ]] in
       do~ [[ return_ ~(| _4, _5 |) ]] in
       M.pure (BlockUnit.Tt, tt)
     in
@@ -69,7 +69,7 @@ Module Erc20_403.
         let~ value := [[ calldataload ~(| 4 |) ]] in
         let_state~ 'tt := [[
           Shallow.if_ (|
-            iszero ~(| (eq ~(| value, (and ~(| value, (sub ~(| (shl ~(| 160, 1 |)), 1 |)) |)) |)) |),
+            iszero ~(| eq ~(| value, and ~(| value, sub ~(| shl ~(| 160, 1 |), 1 |) |) |) |),
             do~ [[ revert ~(| 0, 0 |) ]] in
             M.pure (BlockUnit.Tt, tt),
             tt
@@ -84,7 +84,7 @@ Module Erc20_403.
         let~ value := [[ calldataload ~(| 36 |) ]] in
         let_state~ 'tt := [[
           Shallow.if_ (|
-            iszero ~(| (eq ~(| value, (and ~(| value, (sub ~(| (shl ~(| 160, 1 |)), 1 |)) |)) |)) |),
+            iszero ~(| eq ~(| value, and ~(| value, sub ~(| shl ~(| 160, 1 |), 1 |) |) |) |),
             do~ [[ revert ~(| 0, 0 |) ]] in
             M.pure (BlockUnit.Tt, tt),
             tt
@@ -100,7 +100,7 @@ Module Erc20_403.
         let_state~ 'tt := [[
           Shallow.if_ (|
             gt ~(| x, sum |),
-            do~ [[ mstore ~(| 0, (shl ~(| 224, 0x4e487b71 |)) |) ]] in
+            do~ [[ mstore ~(| 0, shl ~(| 224, 0x4e487b71 |) |) ]] in
             do~ [[ mstore ~(| 4, 0x11 |) ]] in
             do~ [[ revert ~(| 0, 0x24 |) ]] in
             M.pure (BlockUnit.Tt, tt),
@@ -117,7 +117,7 @@ Module Erc20_403.
         let_state~ 'tt := [[
           Shallow.if_ (|
             gt ~(| diff, x |),
-            do~ [[ mstore ~(| 0, (shl ~(| 224, 0x4e487b71 |)) |) ]] in
+            do~ [[ mstore ~(| 0, shl ~(| 224, 0x4e487b71 |) |) ]] in
             do~ [[ mstore ~(| 4, 0x11 |) ]] in
             do~ [[ revert ~(| 0, 0x24 |) ]] in
             M.pure (BlockUnit.Tt, tt),
@@ -130,31 +130,31 @@ Module Erc20_403.
 
     Definition fun_approve (var_owner : U256.t) (var_spender : U256.t) (var_value : U256.t) : M.t unit :=
       let~ '(_, result) :=
-        let~ _1 := [[ and ~(| var_owner, (sub ~(| (shl ~(| 160, 1 |)), 1 |)) |) ]] in
+        let~ _1 := [[ and ~(| var_owner, sub ~(| shl ~(| 160, 1 |), 1 |) |) ]] in
         let_state~ 'tt := [[
           Shallow.if_ (|
             iszero ~(| _1 |),
             let~ memPtr := [[ mload ~(| 64 |) ]] in
-            do~ [[ mstore ~(| memPtr, (shl ~(| 229, 4594637 |)) |) ]] in
-            do~ [[ mstore ~(| (add ~(| memPtr, 4 |)), 32 |) ]] in
-            do~ [[ mstore ~(| (add ~(| memPtr, 36 |)), 36 |) ]] in
-            do~ [[ mstore ~(| (add ~(| memPtr, 68 |)), 0x45726332303a20617070726f76652066726f6d20746865207a65726f20616464 (* Erc20: approve from the zero add *) |) ]] in
-            do~ [[ mstore ~(| (add ~(| memPtr, 100 |)), 0x7265737300000000000000000000000000000000000000000000000000000000 (* ress *) |) ]] in
+            do~ [[ mstore ~(| memPtr, shl ~(| 229, 4594637 |) |) ]] in
+            do~ [[ mstore ~(| add ~(| memPtr, 4 |), 32 |) ]] in
+            do~ [[ mstore ~(| add ~(| memPtr, 36 |), 36 |) ]] in
+            do~ [[ mstore ~(| add ~(| memPtr, 68 |), 0x45726332303a20617070726f76652066726f6d20746865207a65726f20616464 (* Erc20: approve from the zero add *) |) ]] in
+            do~ [[ mstore ~(| add ~(| memPtr, 100 |), 0x7265737300000000000000000000000000000000000000000000000000000000 (* ress *) |) ]] in
             do~ [[ revert ~(| memPtr, 132 |) ]] in
             M.pure (BlockUnit.Tt, tt),
             tt
           |)
         ]] default~ tt in
-        let~ _2 := [[ and ~(| var_spender, (sub ~(| (shl ~(| 160, 1 |)), 1 |)) |) ]] in
+        let~ _2 := [[ and ~(| var_spender, sub ~(| shl ~(| 160, 1 |), 1 |) |) ]] in
         let_state~ 'tt := [[
           Shallow.if_ (|
             iszero ~(| _2 |),
             let~ memPtr_1 := [[ mload ~(| 64 |) ]] in
-            do~ [[ mstore ~(| memPtr_1, (shl ~(| 229, 4594637 |)) |) ]] in
-            do~ [[ mstore ~(| (add ~(| memPtr_1, 4 |)), 32 |) ]] in
-            do~ [[ mstore ~(| (add ~(| memPtr_1, 36 |)), 34 |) ]] in
-            do~ [[ mstore ~(| (add ~(| memPtr_1, 68 |)), 0x45726332303a20617070726f766520746f20746865207a65726f206164647265 (* Erc20: approve to the zero addre *) |) ]] in
-            do~ [[ mstore ~(| (add ~(| memPtr_1, 100 |)), 0x7373000000000000000000000000000000000000000000000000000000000000 (* ss *) |) ]] in
+            do~ [[ mstore ~(| memPtr_1, shl ~(| 229, 4594637 |) |) ]] in
+            do~ [[ mstore ~(| add ~(| memPtr_1, 4 |), 32 |) ]] in
+            do~ [[ mstore ~(| add ~(| memPtr_1, 36 |), 34 |) ]] in
+            do~ [[ mstore ~(| add ~(| memPtr_1, 68 |), 0x45726332303a20617070726f766520746f20746865207a65726f206164647265 (* Erc20: approve to the zero addre *) |) ]] in
+            do~ [[ mstore ~(| add ~(| memPtr_1, 100 |), 0x7373000000000000000000000000000000000000000000000000000000000000 (* ss *) |) ]] in
             do~ [[ revert ~(| memPtr_1, 132 |) ]] in
             M.pure (BlockUnit.Tt, tt),
             tt
@@ -177,34 +177,34 @@ Module Erc20_403.
 
     Definition fun_transfer (var_from : U256.t) (var_to : U256.t) (var_value : U256.t) : M.t unit :=
       let~ '(_, result) :=
-        let~ _1 := [[ and ~(| var_to, (sub ~(| (shl ~(| 160, 1 |)), 1 |)) |) ]] in
+        let~ _1 := [[ and ~(| var_to, sub ~(| shl ~(| 160, 1 |), 1 |) |) ]] in
         let_state~ 'tt := [[
           Shallow.if_ (|
             iszero ~(| _1 |),
             let~ memPtr := [[ mload ~(| 64 |) ]] in
-            do~ [[ mstore ~(| memPtr, (shl ~(| 229, 4594637 |)) |) ]] in
-            do~ [[ mstore ~(| (add ~(| memPtr, 4 |)), 32 |) ]] in
-            do~ [[ mstore ~(| (add ~(| memPtr, 36 |)), 35 |) ]] in
-            do~ [[ mstore ~(| (add ~(| memPtr, 68 |)), 0x45726332303a207472616e7366657220746f20746865207a65726f2061646472 (* Erc20: transfer to the zero addr *) |) ]] in
-            do~ [[ mstore ~(| (add ~(| memPtr, 100 |)), 0x6573730000000000000000000000000000000000000000000000000000000000 (* ess *) |) ]] in
+            do~ [[ mstore ~(| memPtr, shl ~(| 229, 4594637 |) |) ]] in
+            do~ [[ mstore ~(| add ~(| memPtr, 4 |), 32 |) ]] in
+            do~ [[ mstore ~(| add ~(| memPtr, 36 |), 35 |) ]] in
+            do~ [[ mstore ~(| add ~(| memPtr, 68 |), 0x45726332303a207472616e7366657220746f20746865207a65726f2061646472 (* Erc20: transfer to the zero addr *) |) ]] in
+            do~ [[ mstore ~(| add ~(| memPtr, 100 |), 0x6573730000000000000000000000000000000000000000000000000000000000 (* ess *) |) ]] in
             do~ [[ revert ~(| memPtr, 132 |) ]] in
             M.pure (BlockUnit.Tt, tt),
             tt
           |)
         ]] default~ tt in
-        let~ _2 := [[ and ~(| var_from, (sub ~(| (shl ~(| 160, 1 |)), 1 |)) |) ]] in
+        let~ _2 := [[ and ~(| var_from, sub ~(| shl ~(| 160, 1 |), 1 |) |) ]] in
         do~ [[ mstore ~(| 0x00, _2 |) ]] in
         do~ [[ mstore ~(| 0x20, 0x00 |) ]] in
-        let~ _3 := [[ checked_sub_uint256 ~(| (sload ~(| (keccak256 ~(| 0x00, 0x40 |)) |)), var_value |) ]] in
+        let~ _3 := [[ checked_sub_uint256 ~(| sload ~(| keccak256 ~(| 0x00, 0x40 |) |), var_value |) ]] in
         do~ [[ mstore ~(| 0x00, _2 |) ]] in
         do~ [[ mstore ~(| 0x20, 0x00 |) ]] in
-        do~ [[ sstore ~(| (keccak256 ~(| 0x00, 0x40 |)), _3 |) ]] in
+        do~ [[ sstore ~(| keccak256 ~(| 0x00, 0x40 |), _3 |) ]] in
         do~ [[ mstore ~(| 0x00, _1 |) ]] in
         do~ [[ mstore ~(| 0x20, 0x00 |) ]] in
-        let~ _4 := [[ checked_add_uint256 ~(| (sload ~(| (keccak256 ~(| 0x00, 0x40 |)) |)), var_value |) ]] in
+        let~ _4 := [[ checked_add_uint256 ~(| sload ~(| keccak256 ~(| 0x00, 0x40 |) |), var_value |) ]] in
         do~ [[ mstore ~(| 0x00, _1 |) ]] in
         do~ [[ mstore ~(| 0x20, 0x00 |) ]] in
-        do~ [[ sstore ~(| (keccak256 ~(| 0x00, 0x40 |)), _4 |) ]] in
+        do~ [[ sstore ~(| keccak256 ~(| 0x00, 0x40 |), _4 |) ]] in
         let~ _5 := [[ mload ~(| 0x40 |) ]] in
         do~ [[ mstore ~(| _5, var_value |) ]] in
         do~ [[ log3 ~(| _5, 0x20, 0xddf252ad1be2c89b69c2b068fc378daa952ba7f163c4a11628f55a4df523b3ef, _2, _1 |) ]] in
@@ -214,13 +214,13 @@ Module Erc20_403.
 
     Definition body : M.t unit :=
       do~
-        do~ [[ mstore ~(| 64, (memoryguard ~(| 0x80 |)) |) ]] in
+        do~ [[ mstore ~(| 64, memoryguard ~(| 0x80 |) |) ]] in
         let_state~ 'tt := [[
           Shallow.if_ (|
-            iszero ~(| (lt ~(| (calldatasize ~(||)), 4 |)) |),
+            iszero ~(| lt ~(| calldatasize ~(||), 4 |) |),
             let_state~ 'tt := [[
               (* switch *)
-              let~ δ := [[ shr ~(| 224, (calldataload ~(| 0 |)) |) ]] in
+              let~ δ := [[ shr ~(| 224, calldataload ~(| 0 |) |) ]] in
               if δ =? 0x095ea7b3 then
                 let_state~ 'tt := [[
                   Shallow.if_ (|
@@ -232,14 +232,14 @@ Module Erc20_403.
                 ]] default~ tt in
                 let_state~ 'tt := [[
                   Shallow.if_ (|
-                    slt ~(| (add ~(| (calldatasize ~(||)), (not ~(| 3 |)) |)), 64 |),
+                    slt ~(| add ~(| calldatasize ~(||), not ~(| 3 |) |), 64 |),
                     do~ [[ revert ~(| 0, 0 |) ]] in
                     M.pure (BlockUnit.Tt, tt),
                     tt
                   |)
                 ]] default~ tt in
                 let~ value0 := [[ abi_decode_address ~(||) ]] in
-                do~ [[ fun_approve ~(| (caller ~(||)), value0, (calldataload ~(| 36 |)) |) ]] in
+                do~ [[ fun_approve ~(| caller ~(||), value0, calldataload ~(| 36 |) |) ]] in
                 let~ memPos := [[ mload ~(| 64 |) ]] in
                 do~ [[ mstore ~(| memPos, 1 |) ]] in
                 do~ [[ return_ ~(| memPos, 32 |) ]] in
@@ -255,7 +255,7 @@ Module Erc20_403.
                 ]] default~ tt in
                 let_state~ 'tt := [[
                   Shallow.if_ (|
-                    slt ~(| (add ~(| (calldatasize ~(||)), (not ~(| 3 |)) |)), 0 |),
+                    slt ~(| add ~(| calldatasize ~(||), not ~(| 3 |) |), 0 |),
                     do~ [[ revert ~(| 0, 0 |) ]] in
                     M.pure (BlockUnit.Tt, tt),
                     tt
@@ -277,7 +277,7 @@ Module Erc20_403.
                 ]] default~ tt in
                 let_state~ 'tt := [[
                   Shallow.if_ (|
-                    slt ~(| (add ~(| (calldatasize ~(||)), (not ~(| 3 |)) |)), 96 |),
+                    slt ~(| add ~(| calldatasize ~(||), not ~(| 3 |) |), 96 |),
                     do~ [[ revert ~(| 0, 0 |) ]] in
                     M.pure (BlockUnit.Tt, tt),
                     tt
@@ -287,14 +287,14 @@ Module Erc20_403.
                 let~ value1 := [[ abi_decode_address_2305 ~(||) ]] in
                 let~ value := [[ calldataload ~(| 68 |) ]] in
                 do~ [[ fun_transfer ~(| value0_1, value1, value |) ]] in
-                do~ [[ mstore ~(| 0, (and ~(| value0_1, (sub ~(| (shl ~(| 160, 1 |)), 1 |)) |)) |) ]] in
+                do~ [[ mstore ~(| 0, and ~(| value0_1, sub ~(| shl ~(| 160, 1 |), 1 |) |) |) ]] in
                 do~ [[ mstore ~(| 32, 1 |) ]] in
                 let~ dataSlot := [[ keccak256 ~(| 0, 64 |) ]] in
                 let~ dataSlot_1 := [[ 0 ]] in
-                do~ [[ mstore ~(| 0, (and ~(| (caller ~(||)), (sub ~(| (shl ~(| 160, 1 |)), 1 |)) |)) |) ]] in
+                do~ [[ mstore ~(| 0, and ~(| caller ~(||), sub ~(| shl ~(| 160, 1 |), 1 |) |) |) ]] in
                 do~ [[ mstore ~(| 0x20, dataSlot |) ]] in
                 let~ dataSlot_1 := [[ keccak256 ~(| 0, 0x40 |) ]] in
-                do~ [[ fun_approve ~(| value0_1, (caller ~(||)), (checked_sub_uint256 ~(| (sload ~(| dataSlot_1 |)), value |)) |) ]] in
+                do~ [[ fun_approve ~(| value0_1, caller ~(||), checked_sub_uint256 ~(| sload ~(| dataSlot_1 |), value |) |) ]] in
                 let~ memPos_2 := [[ mload ~(| 64 |) ]] in
                 do~ [[ mstore ~(| memPos_2, 1 |) ]] in
                 do~ [[ return_ ~(| memPos_2, 32 |) ]] in
@@ -310,21 +310,21 @@ Module Erc20_403.
                 ]] default~ tt in
                 let_state~ 'tt := [[
                   Shallow.if_ (|
-                    slt ~(| (add ~(| (calldatasize ~(||)), (not ~(| 3 |)) |)), 64 |),
+                    slt ~(| add ~(| calldatasize ~(||), not ~(| 3 |) |), 64 |),
                     do~ [[ revert ~(| 0, 0 |) ]] in
                     M.pure (BlockUnit.Tt, tt),
                     tt
                   |)
                 ]] default~ tt in
                 let~ value0_2 := [[ abi_decode_address ~(||) ]] in
-                do~ [[ mstore ~(| 0, (caller ~(||)) |) ]] in
+                do~ [[ mstore ~(| 0, caller ~(||) |) ]] in
                 do~ [[ mstore ~(| 32, 1 |) ]] in
                 let~ dataSlot_2 := [[ keccak256 ~(| 0, 64 |) ]] in
                 let~ dataSlot_3 := [[ 0 ]] in
-                do~ [[ mstore ~(| 0, (and ~(| value0_2, (sub ~(| (shl ~(| 160, 1 |)), 1 |)) |)) |) ]] in
+                do~ [[ mstore ~(| 0, and ~(| value0_2, sub ~(| shl ~(| 160, 1 |), 1 |) |) |) ]] in
                 do~ [[ mstore ~(| 0x20, dataSlot_2 |) ]] in
                 let~ dataSlot_3 := [[ keccak256 ~(| 0, 0x40 |) ]] in
-                do~ [[ fun_approve ~(| (caller ~(||)), value0_2, (checked_add_uint256 ~(| (sload ~(| dataSlot_3 |)), (calldataload ~(| 36 |)) |)) |) ]] in
+                do~ [[ fun_approve ~(| caller ~(||), value0_2, checked_add_uint256 ~(| sload ~(| dataSlot_3 |), calldataload ~(| 36 |) |) |) ]] in
                 let~ memPos_3 := [[ mload ~(| 64 |) ]] in
                 do~ [[ mstore ~(| memPos_3, 1 |) ]] in
                 do~ [[ return_ ~(| memPos_3, 32 |) ]] in
@@ -340,15 +340,15 @@ Module Erc20_403.
                 ]] default~ tt in
                 let_state~ 'tt := [[
                   Shallow.if_ (|
-                    slt ~(| (add ~(| (calldatasize ~(||)), (not ~(| 3 |)) |)), 32 |),
+                    slt ~(| add ~(| calldatasize ~(||), not ~(| 3 |) |), 32 |),
                     do~ [[ revert ~(| 0, 0 |) ]] in
                     M.pure (BlockUnit.Tt, tt),
                     tt
                   |)
                 ]] default~ tt in
-                do~ [[ mstore ~(| 0, (and ~(| (abi_decode_address ~(||)), (sub ~(| (shl ~(| 160, 1 |)), 1 |)) |)) |) ]] in
+                do~ [[ mstore ~(| 0, and ~(| abi_decode_address ~(||), sub ~(| shl ~(| 160, 1 |), 1 |) |) |) ]] in
                 do~ [[ mstore ~(| 32, 0 |) ]] in
-                let~ _2 := [[ sload ~(| (keccak256 ~(| 0, 64 |)) |) ]] in
+                let~ _2 := [[ sload ~(| keccak256 ~(| 0, 64 |) |) ]] in
                 let~ memPos_4 := [[ mload ~(| 64 |) ]] in
                 do~ [[ mstore ~(| memPos_4, _2 |) ]] in
                 do~ [[ return_ ~(| memPos_4, 32 |) ]] in
@@ -364,21 +364,21 @@ Module Erc20_403.
                 ]] default~ tt in
                 let_state~ 'tt := [[
                   Shallow.if_ (|
-                    slt ~(| (add ~(| (calldatasize ~(||)), (not ~(| 3 |)) |)), 64 |),
+                    slt ~(| add ~(| calldatasize ~(||), not ~(| 3 |) |), 64 |),
                     do~ [[ revert ~(| 0, 0 |) ]] in
                     M.pure (BlockUnit.Tt, tt),
                     tt
                   |)
                 ]] default~ tt in
                 let~ value0_3 := [[ abi_decode_address ~(||) ]] in
-                do~ [[ mstore ~(| 0, (caller ~(||)) |) ]] in
+                do~ [[ mstore ~(| 0, caller ~(||) |) ]] in
                 do~ [[ mstore ~(| 32, 1 |) ]] in
                 let~ dataSlot_4 := [[ keccak256 ~(| 0, 64 |) ]] in
                 let~ dataSlot_5 := [[ 0 ]] in
-                do~ [[ mstore ~(| 0, (and ~(| value0_3, (sub ~(| (shl ~(| 160, 1 |)), 1 |)) |)) |) ]] in
+                do~ [[ mstore ~(| 0, and ~(| value0_3, sub ~(| shl ~(| 160, 1 |), 1 |) |) |) ]] in
                 do~ [[ mstore ~(| 0x20, dataSlot_4 |) ]] in
                 let~ dataSlot_5 := [[ keccak256 ~(| 0, 0x40 |) ]] in
-                do~ [[ fun_approve ~(| (caller ~(||)), value0_3, (checked_sub_uint256 ~(| (sload ~(| dataSlot_5 |)), (calldataload ~(| 36 |)) |)) |) ]] in
+                do~ [[ fun_approve ~(| caller ~(||), value0_3, checked_sub_uint256 ~(| sload ~(| dataSlot_5 |), calldataload ~(| 36 |) |) |) ]] in
                 let~ memPos_5 := [[ mload ~(| 64 |) ]] in
                 do~ [[ mstore ~(| memPos_5, 1 |) ]] in
                 do~ [[ return_ ~(| memPos_5, 32 |) ]] in
@@ -394,14 +394,14 @@ Module Erc20_403.
                 ]] default~ tt in
                 let_state~ 'tt := [[
                   Shallow.if_ (|
-                    slt ~(| (add ~(| (calldatasize ~(||)), (not ~(| 3 |)) |)), 64 |),
+                    slt ~(| add ~(| calldatasize ~(||), not ~(| 3 |) |), 64 |),
                     do~ [[ revert ~(| 0, 0 |) ]] in
                     M.pure (BlockUnit.Tt, tt),
                     tt
                   |)
                 ]] default~ tt in
                 let~ value0_4 := [[ abi_decode_address ~(||) ]] in
-                do~ [[ fun_transfer ~(| (caller ~(||)), value0_4, (calldataload ~(| 36 |)) |) ]] in
+                do~ [[ fun_transfer ~(| caller ~(||), value0_4, calldataload ~(| 36 |) |) ]] in
                 let~ memPos_6 := [[ mload ~(| 64 |) ]] in
                 do~ [[ mstore ~(| memPos_6, 1 |) ]] in
                 do~ [[ return_ ~(| memPos_6, 32 |) ]] in
@@ -417,7 +417,7 @@ Module Erc20_403.
                 ]] default~ tt in
                 let_state~ 'tt := [[
                   Shallow.if_ (|
-                    slt ~(| (add ~(| (calldatasize ~(||)), (not ~(| 3 |)) |)), 64 |),
+                    slt ~(| add ~(| calldatasize ~(||), not ~(| 3 |) |), 64 |),
                     do~ [[ revert ~(| 0, 0 |) ]] in
                     M.pure (BlockUnit.Tt, tt),
                     tt
@@ -425,11 +425,11 @@ Module Erc20_403.
                 ]] default~ tt in
                 let~ value0_5 := [[ abi_decode_address ~(||) ]] in
                 let~ value1_1 := [[ abi_decode_address_2305 ~(||) ]] in
-                do~ [[ mstore ~(| 0, (and ~(| value0_5, (sub ~(| (shl ~(| 160, 1 |)), 1 |)) |)) |) ]] in
+                do~ [[ mstore ~(| 0, and ~(| value0_5, sub ~(| shl ~(| 160, 1 |), 1 |) |) |) ]] in
                 do~ [[ mstore ~(| 32, 0x01 |) ]] in
                 let~ dataSlot_6 := [[ keccak256 ~(| 0, 64 |) ]] in
                 let~ dataSlot_7 := [[ 0 ]] in
-                do~ [[ mstore ~(| 0, (and ~(| value1_1, (sub ~(| (shl ~(| 160, 1 |)), 1 |)) |)) |) ]] in
+                do~ [[ mstore ~(| 0, and ~(| value1_1, sub ~(| shl ~(| 160, 1 |), 1 |) |) |) ]] in
                 do~ [[ mstore ~(| 0x20, dataSlot_6 |) ]] in
                 let~ dataSlot_7 := [[ keccak256 ~(| 0, 0x40 |) ]] in
                 let~ _3 := [[ sload ~(| dataSlot_7 |) ]] in
