coq/CoqOfSolidity/contracts/erc20/proofs/erc20.v
@@ -8,31 +8,6 @@ Import RunO.
 
 Ltac Zify.zify_post_hook ::= Z.to_euclidean_division_equations.
 
-(** Apply the [simpl] tactic on the expressions of the reduction relation, the finale state, but not
-    the initial state. *)
-Ltac simpl_goal :=
-  match goal with
-  | |- {{? _, _, _ | ?expr1 ⇓ ?expr2 | ?state_end ?}} =>
-    let expr1' := eval simpl in expr1 in
-    change expr1 with expr1';
-    let expr2' := eval simpl in expr2 in
-    change expr2 with expr2';
-    let state_end' := eval simpl in state_end in
-    change state_end with state_end'
-  end.
-
-(** ** Very short shortcuts for commonly used tactics. *)
-Ltac p := apply RunO.Pure.
-Ltac pn := apply RunO.PureNone.
-Ltac pe := apply RunO.PureEq.
-Ltac pr := eapply RunO.Primitive; [reflexivity |].
-Ltac prn := eapply RunO.PrimitiveNone.
-Ltac l := eapply RunO.Let.
-Ltac lu := apply RunO.LetUnfold.
-Ltac c := eapply RunO.Call.
-Ltac cu := apply RunO.CallUnfold.
-Ltac s := fold @LowM.let_; simpl_goal.
-
 Opaque StdlibAux.keccak256.
 
 (** Direct proofs of elements of the `erc20.v` file. *)
@@ -780,13 +755,6 @@ Module Erc20_403.
         Result.Revert 0 0x24
       else
         Result.Ok (x - y).
-
-    Definition wrap_state_with_revert {A : Set} (state : State.t) (output : Result.t A) :
-        option State.t :=
-      match output with
-      | Result.Revert _ _ => None
-      | _ => Some state
-      end.
 
     Lemma run_checked_sub_uint256 codes environment state
         (x y : U256.t) :
